Use modules, simp, grind in Atoms

ExistentialRules/AtomsAndFacts/Basic.lean
@@ -1,9 +1,11 @@
+module
+
 import BasicLeanDatastructures.List.Basic
 import BasicLeanDatastructures.List.EraseDupsKeepRight
-import BasicLeanDatastructures.Set.Basic
-import BasicLeanDatastructures.Set.Finite
+public import BasicLeanDatastructures.Set.Basic
+public import BasicLeanDatastructures.Set.Finite
 
-import ExistentialRules.Terms.Basic
+public import ExistentialRules.Terms.Basic
 import ExistentialRules.Terms.ListsOfTerms
 
 /-!
@@ -15,6 +17,8 @@ This includes first and foremost `Atom` and `Fact` but also
 
 The atom-like datastructures are all expressed in terms of a `GeneralizedAtom`. This will turn out convenient when defining substitutions and homomorphisms next since these can (for the most part) just be defines as generic mapping over `GeneralizedAtom`.
 -/
+
+public section
 
 /-- A `GeneralizedAtom` consists of a predicate symbol and a list of terms of an arbitrary type such that the number of terms matches the predicate's arity. -/
 structure GeneralizedAtom (sig : Signature) (T : Type u) [DecidableEq sig.P] where
@@ -57,29 +61,28 @@ def skolemize (ruleId : Nat) (disjunctIndex : Nat) (frontier : List sig.V) (a : 
 }
 
 /-- A variable occurs in `variables` iff it is a term of the `FunctionFreeAtom. -/
+@[simp, grind =]
 theorem mem_variables {a : FunctionFreeAtom sig} {v : sig.V} : v ∈ a.variables ↔ (VarOrConst.var v) ∈ a.terms := by
-  constructor
-  . intro v_mem; apply VarOrConst.filterVars_occur_in_original_list; exact v_mem
-  . intro v_mem; apply VarOrConst.mem_filterVars_of_var; exact v_mem
+  unfold variables; grind
 
 /-- A constant occurs in `constants` iff it is a term of the `FunctionFreeAtom. -/
+@[simp, grind =]
 theorem mem_constants {a : FunctionFreeAtom sig} {c : sig.C} : c ∈ a.constants ↔ (VarOrConst.const c) ∈ a.terms := by
-  constructor
-  . intro c_mem; apply VarOrConst.filterConsts_occur_in_original_list; exact c_mem
-  . intro c_mem; apply VarOrConst.mem_filterConsts_of_const; exact c_mem
+  unfold constants; grind
 
 /-- The number of terms remains unchanged when Skolemizing. -/
+@[simp, grind =]
 theorem length_skolemize {ruleId : Nat} {disjunctIndex : Nat} {frontier : List sig.V} {a : FunctionFreeAtom sig} :
     (a.skolemize ruleId disjunctIndex frontier).terms.length = a.terms.length := by
-  unfold skolemize
-  rw [List.length_map]
+  unfold skolemize; simp
 
 /-- If a a `VarOrConst` occurs in the terms of the `FunctionFreeAtom`, then the Skolemized `VarOrConst` occurs in the Skolemized `Atom`. -/
+@[grind <-]
 theorem mem_skolemize_of_mem {ruleId : Nat} {disjunctIndex : Nat} {frontier : List sig.V}
     {a : FunctionFreeAtom sig} {t : VarOrConst sig} :
     t ∈ a.terms -> (t.skolemize ruleId disjunctIndex frontier) ∈ (a.skolemize ruleId disjunctIndex frontier).terms := by
-  intro t_mem
   unfold skolemize
+  intro t_mem
   rw [List.mem_map]
   exists t
 
@@ -101,6 +104,7 @@ namespace FunctionFreeConjunction
 variable {sig : Signature} [DecidableEq sig.P] [DecidableEq sig.C] [DecidableEq sig.V]
 
 /-- The `terms` of a `FunctionFreeConjunction` are the terms of all its atoms. -/
+@[expose]
 def terms (conj : FunctionFreeConjunction sig) : List (VarOrConst sig) := conj.flatMap GeneralizedAtom.terms
 
 /-- The `vars` of a `FunctionFreeConjunction` are the variables of all its atoms. -/
@@ -110,23 +114,20 @@ def vars (conj : FunctionFreeConjunction sig) : List sig.V := conj.flatMap Funct
 def consts (conj : FunctionFreeConjunction sig) : List sig.C := conj.flatMap FunctionFreeAtom.constants
 
 /-- The `predicates` of a `FunctionFreeConjunction` are the predicates of all its atoms. -/
+@[expose]
 def predicates (conj : FunctionFreeConjunction sig) : List sig.P := conj.map GeneralizedAtom.predicate
 
 /-- Different from the definition, we can also say that a variable is in `variables` iff there is a `FunctionFreeAtom` in the conjunction that features the variable as a term. -/
+@[simp, grind =]
 theorem mem_vars {conj : FunctionFreeConjunction sig} {v : sig.V} :
     v ∈ conj.vars ↔ ∃ f, f ∈ conj ∧ (VarOrConst.var v) ∈ f.terms := by
-  unfold vars; rw [List.mem_flatMap]
-  constructor
-  . rintro ⟨f, f_mem, v_mem⟩; exists f; constructor; exact f_mem; rw [← FunctionFreeAtom.mem_variables]; exact v_mem
-  . rintro ⟨f, f_mem, v_mem⟩; exists f; constructor; exact f_mem; rw [FunctionFreeAtom.mem_variables]; exact v_mem
+  unfold vars; simp
 
 /-- Different from the definition, we can also say that a constant is in `constants` iff there is a `FunctionFreeAtom` in the conjunction that features the constant as a term. -/
+@[simp, grind =]
 theorem mem_consts {conj : FunctionFreeConjunction sig} {c : sig.C} :
     c ∈ conj.consts ↔ ∃ f, f ∈ conj ∧ (VarOrConst.const c) ∈ f.terms := by
-  unfold consts; rw [List.mem_flatMap]
-  constructor
-  . rintro ⟨f, f_mem, c_mem⟩; exists f; constructor; exact f_mem; rw [← FunctionFreeAtom.mem_constants]; exact c_mem
-  . rintro ⟨f, f_mem, c_mem⟩; exists f; constructor; exact f_mem; rw [FunctionFreeAtom.mem_constants]; exact c_mem
+  unfold consts; simp
 
 end FunctionFreeConjunction
 
@@ -159,85 +160,83 @@ namespace Rule
 variable {sig : Signature} [DecidableEq sig.P] [DecidableEq sig.C] [DecidableEq sig.V]
 
 /-- This function returns the frontier variables that occur in a given head disjunct. This is a sublist of all the frontier variables. -/
-def frontier_for_head (r : Rule sig) (i : Fin r.head.length) : List sig.V :=
-  r.body.vars.filter (fun v => v ∈ r.head[i.val].vars)
+@[expose]
+def frontier_for_head (r : Rule sig) (i : Nat) (lt : i < r.head.length) : List sig.V :=
+  r.body.vars.filter (fun v => v ∈ r.head[i].vars)
 
 /-- This returns all the `frontier` variables of the rule, i.e. the variables that occur in both body and some head. -/
+@[expose]
 def frontier (r : Rule sig) : List sig.V :=
   r.body.vars.filter (fun v => r.head.any (fun h => v ∈ h.vars))
 
 /-- The `pure_body_vars` are the variables from the body that are not in the `frontier`. -/
+@[expose]
 def pure_body_vars (r : Rule sig) : List sig.V := r.body.vars.filter (fun x => x ∉ r.frontier)
 
 /-- We call a rule `isDatalog` if it does not contain existential variables, i.e. if all head variables occur in the body. -/
+@[expose]
 def isDatalog (r : Rule sig) : Bool :=
   r.head.all (fun h => h.vars.all (fun v => v ∈ r.body.vars))
 
 /-- We call a rule `isDeterministic` if it has exactly one head disjunct. -/
+@[expose]
 def isDeterministic (r : Rule sig) : Bool := r.head.length = 1
 
 /-- The predicate symbols of a rule are just the predicate symbols from the body and all heads. -/
+@[expose]
 def predicates (r : Rule sig) : List sig.P := r.body.predicates ++ (r.head.flatMap FunctionFreeConjunction.predicates)
 
 /-- The constants of a rule are just the constants from the body and all heads. -/
+@[expose]
 def constants (r : Rule sig) : List sig.C := r.body.consts ++ r.head.flatMap (fun conj => conj.consts)
 
 /-- Sometimes we require only the constants from the heads and therefore we define them here. -/
+@[expose]
 def head_constants (r : Rule sig) : List sig.C := r.head.flatMap (fun conj => conj.consts)
 
 /-- The existential variables for a given head are simply the variables from the head that are not in the frontier. -/
+@[expose]
 def existential_vars_for_head_disjunct (r : Rule sig) (i : Nat) (lt : i < r.head.length) : List sig.V :=
   r.head[i].vars.filter (fun v => v ∉ r.frontier)
 
 /-- The Skolem function symbols of a rule are all `SkolemFS` with the rule id, all possible head indices and the respective existential variables. -/
+@[expose]
 def skolem_functions (r : Rule sig) : List (SkolemFS sig) := r.head.zipIdx.flatMap (fun (head, i) =>
   (head.vars.filter (fun v => v ∉ r.frontier)).map (fun v => { ruleId := r.id, disjunctIndex := i, var := v, arity := r.frontier.length })
 )
 
 /-- A variable is a frontier variable if and only if it is a frontier variable in some head disjunct. -/
 theorem mem_frontier_iff_mem_frontier_for_head {r : Rule sig} {v : sig.V} :
-    v ∈ r.frontier ↔ ∃ i, v ∈ r.frontier_for_head i := by
-  unfold frontier frontier_for_head; simp only [List.mem_filter, List.any_eq_true, decide_eq_true_iff]
+    v ∈ r.frontier ↔ ∃ i lt, v ∈ r.frontier_for_head i lt := by
+  unfold frontier frontier_for_head
+  simp only [List.mem_filter, List.any_eq_true, decide_eq_true_iff]
   constructor
   . rintro ⟨mem_body, ⟨h, h_mem, mem_h⟩⟩
     rw [List.mem_iff_getElem] at h_mem
-    rcases h_mem with ⟨i, lt, h_mem⟩
-    exists ⟨i, lt⟩
-    constructor
-    . exact mem_body
-    . rw [h_mem]; exact mem_h
-  . rintro ⟨⟨i, lt⟩, mem_body, mem_h⟩
-    constructor
-    . exact mem_body
-    . exists r.head[i]; constructor; apply List.getElem_mem; exact mem_h
+    grind
+  . grind
 
 /-- A variable is in the frontier of a head if it is in the frontier of the rule and occurs as a term in the given head. -/
-theorem mem_frontier_for_head_of_mem_frontier_of_mem_head_terms {r : Rule sig} {v : sig.V} {i : Fin r.head.length} :
-    v ∈ r.frontier -> VarOrConst.var v ∈ r.head[i.val].terms -> v ∈ r.frontier_for_head i := by
+theorem mem_frontier_for_head_of_mem_frontier_of_mem_head_terms {r : Rule sig} {v : sig.V} {i : Nat} (lt : i < r.head.length) :
+    v ∈ r.frontier -> VarOrConst.var v ∈ r.head[i].terms -> v ∈ r.frontier_for_head i lt := by
   unfold frontier frontier_for_head
-  simp only [List.mem_filter, List.any_eq_true, decide_eq_true_iff]
-  rintro ⟨mem_body, _⟩ mem_head_terms
-  constructor
-  . exact mem_body
-  . unfold FunctionFreeConjunction.terms at mem_head_terms
-    rw [List.mem_flatMap] at mem_head_terms
-    rcases mem_head_terms with ⟨a, a_mem, mem_a⟩
-    rw [FunctionFreeConjunction.mem_vars]; exists a
+  unfold FunctionFreeConjunction.terms
+  grind
 
 /-- All frontier variables occur in the body. -/
+@[grind <-]
 theorem frontier_subset_vars_body {r : Rule sig} : r.frontier ⊆ r.body.vars := by
-  intro v v_mem
-  unfold Rule.frontier at v_mem; rw [List.mem_filter] at v_mem
-  exact v_mem.left
+  unfold Rule.frontier
+  grind
 
 /-- The frontier variables in a given head occur in the list of variables for the same head. -/
-theorem frontier_for_head_subset_vars_head {r : Rule sig} {i : Nat} {lt : i < r.head.length} : r.frontier_for_head ⟨i, lt⟩ ⊆ r.head[i].vars := by
-  intro v v_mem
-  unfold Rule.frontier_for_head at v_mem; rw [List.mem_filter] at v_mem
-  rw [decide_eq_true_iff] at v_mem
-  exact v_mem.right
+@[grind <-]
+theorem frontier_for_head_subset_vars_head {r : Rule sig} {i : Nat} (lt : i < r.head.length) : r.frontier_for_head i lt ⊆ r.head[i].vars := by
+  unfold Rule.frontier_for_head
+  grind
 
 /-- The head constants of the rule are also constants of the whole rule. -/
+@[grind <-]
 theorem head_constants_subset_constants (r : Rule sig) : r.head_constants ⊆ r.constants := by apply List.subset_append_right
 
 end Rule
@@ -269,21 +268,27 @@ namespace RuleSet
 variable {sig : Signature} [DecidableEq sig.P] [DecidableEq sig.C] [DecidableEq sig.V]
 
 /-- A `RuleSet` is is deterministic if each rule is. -/
+@[expose]
 def isDeterministic (rs : RuleSet sig) : Prop := ∀ (r : Rule sig), r ∈ rs.rules -> r.isDeterministic
 
 /-- The predicate symbols of a `RuleSet` are the predicate symbols from all rules. -/
+@[expose]
 def predicates (rs : RuleSet sig) : Set sig.P := fun p => ∃ r, r ∈ rs.rules ∧ p ∈ r.predicates
 
 /-- The constants of a `RuleSet` are the constants from all rules. -/
+@[expose]
 def constants (rs : RuleSet sig) : Set sig.C := fun c => ∃ r, r ∈ rs.rules ∧ c ∈ r.constants
 
 /-- The head constants of a `RuleSet` are the head constants from all rules. -/
+@[expose]
 def head_constants (rs : RuleSet sig) : Set sig.C := fun c => ∃ r, r ∈ rs.rules ∧ c ∈ r.head_constants
 
 /-- The Skolem function symbols of a `RuleSet` are the Skolem function symbols from all rules. -/
+@[expose]
 def skolem_functions (rs : RuleSet sig) : Set (SkolemFS sig) := fun f => ∃ r, r ∈ rs.rules ∧ f ∈ r.skolem_functions
 
 /-- If the `RuleSet` is finite, so are the `predicates`. -/
+@[grind ->]
 theorem predicates_finite_of_finite (rs : RuleSet sig) : rs.rules.finite -> rs.predicates.finite := by
   intro finite
   rcases finite with ⟨l, nodup, eq⟩
@@ -294,11 +299,10 @@ theorem predicates_finite_of_finite (rs : RuleSet sig) : rs.rules.finite -> rs.p
     rw [List.mem_eraseDupsKeepRight]
     unfold predicates
     simp only [List.mem_flatMap]
-    constructor <;> (intro h; rcases h with ⟨r, h⟩; exists r)
-    . rw [← eq]; assumption
-    . rw [eq]; assumption
+    constructor <;> (intro ⟨r, h⟩; exists r; grind)
 
 /-- If the `RuleSet` is finite, so are the `constants`. -/
+@[grind ->]
 theorem constants_finite_of_finite (rs : RuleSet sig) : rs.rules.finite -> rs.constants.finite := by
   intro finite
   rcases finite with ⟨l, nodup, eq⟩
@@ -309,11 +313,10 @@ theorem constants_finite_of_finite (rs : RuleSet sig) : rs.rules.finite -> rs.co
     rw [List.mem_eraseDupsKeepRight]
     unfold constants
     simp only [List.mem_flatMap]
-    constructor <;> (intro h; rcases h with ⟨r, h⟩; exists r)
-    . rw [← eq]; assumption
-    . rw [eq]; assumption
+    constructor <;> (intro ⟨r, h⟩; exists r; grind)
 
 /-- If the `RuleSet` is finite, so are the `head_constants`. -/
+@[grind ->]
 theorem head_constants_finite_of_finite (rs : RuleSet sig) : rs.rules.finite -> rs.head_constants.finite := by
   intro finite
   rcases finite with ⟨l, nodup, eq⟩
@@ -324,11 +327,10 @@ theorem head_constants_finite_of_finite (rs : RuleSet sig) : rs.rules.finite -> 
     rw [List.mem_eraseDupsKeepRight]
     unfold head_constants
     simp only [List.mem_flatMap]
-    constructor <;> (intro h; rcases h with ⟨r, h⟩; exists r)
-    . rw [← eq]; assumption
-    . rw [eq]; assumption
+    constructor <;> (intro ⟨r, h⟩; exists r; grind)
 
 /-- If the `RuleSet` is finite, so are the `skolem_functions`. -/
+@[grind ->]
 theorem skolem_functions_finite_of_finite (rs : RuleSet sig) : rs.rules.finite -> rs.skolem_functions.finite := by
   intro finite
   rcases finite with ⟨l, nodup, eq⟩
@@ -339,11 +341,10 @@ theorem skolem_functions_finite_of_finite (rs : RuleSet sig) : rs.rules.finite -
     rw [List.mem_eraseDupsKeepRight]
     unfold skolem_functions
     simp only [List.mem_flatMap]
-    constructor <;> (intro h; rcases h with ⟨r, h⟩; exists r)
-    . rw [← eq]; assumption
-    . rw [eq]; assumption
+    constructor <;> (intro ⟨r, h⟩; exists r; grind)
 
 /-- The `head_constants` of a `RuleSet` are a subset of the `constants`. -/
+@[grind <-]
 theorem head_constants_subset_constants (rs : RuleSet sig) : rs.head_constants ⊆ rs.constants := by
   intro c c_mem
   rcases c_mem with ⟨r, r_mem, c_mem⟩
@@ -367,9 +368,11 @@ def get_by_id (rl : RuleList sig) (id : Nat) (id_mem : ∃ r ∈ rl.rules, r.id 
   (rl.rules.find? (fun r => r.id = id)).get (by simp [id_mem])
 
 /-- A rule that we get by id is in the `RuleList`. -/
-theorem get_by_id_mem (rl : RuleList sig) (id : Nat) (id_mem : ∃ r ∈ rl.rules, r.id = id) : rl.get_by_id id id_mem ∈ rl.rules := by unfold get_by_id; apply List.get_find?_mem
+theorem get_by_id_mem (rl : RuleList sig) (id : Nat) (id_mem : ∃ r ∈ rl.rules, r.id = id) : rl.get_by_id id id_mem ∈ rl.rules := by
+  unfold get_by_id; apply List.get_find?_mem
 
 /-- A rule that we get by id is indeed the rule that the id belongs to. -/
+@[simp, grind =]
 theorem get_by_id_self (rl : RuleList sig) (r : Rule sig) (mem : r ∈ rl.rules) : rl.get_by_id r.id (by exists r) = r := by
   apply rl.id_unique
   constructor
@@ -402,15 +405,19 @@ namespace Fact
 variable {sig : Signature} [DecidableEq sig.P] [DecidableEq sig.C] [DecidableEq sig.V]
 
 /-- The `constants` of a `Fact` are the constants of all terms. -/
+@[expose]
 def constants (f : Fact sig) : List sig.C := f.terms.flatMap GroundTerm.constants
 
 /-- The `function_symbols` of a `Fact` are the function symbols of all terms. -/
+@[expose]
 def function_symbols (f : Fact sig) : List (SkolemFS sig) := f.terms.flatMap GroundTerm.functions
 
 /-- A `Fact` is function free, if each term is a constant. -/
+@[expose]
 def isFunctionFree (f : Fact sig) : Prop := ∀ t, t ∈ f.terms -> ∃ c, t = GroundTerm.const c
 
 /-- If a `Fact` `isFunctionFree`, then we can convert it to a `FunctionFreeFact`. -/
+@[expose]
 def toFunctionFreeFact (f : Fact sig) (isFunctionFree : f.isFunctionFree) : FunctionFreeFact sig := {
   predicate := f.predicate
   terms := f.terms.attach.map (fun t => t.val.toConst (isFunctionFree t.val t.property))
@@ -424,6 +431,7 @@ namespace FunctionFreeFact
 variable {sig : Signature} [DecidableEq sig.P] [DecidableEq sig.C] [DecidableEq sig.V]
 
 /-- A `FunctionFreeFact` can always be converted to a `Fact`. -/
+@[expose]
 def toFact (f : FunctionFreeFact sig) : Fact sig := {
   predicate := f.predicate,
   terms := f.terms.map GroundTerm.const,
@@ -431,15 +439,14 @@ def toFact (f : FunctionFreeFact sig) : Fact sig := {
 }
 
 /-- A `Fact` obtained from a `FunctionFreeFact` `isFunctionFree`. -/
+@[grind <-]
 theorem toFact_isFunctionFree (f : FunctionFreeFact sig) : f.toFact.isFunctionFree := by
-  intro t t_mem
-  unfold toFact at t_mem
-  simp at t_mem
-  rcases t_mem with ⟨c, _, t_eq⟩
-  exists c
-  rw [t_eq]
+  intro _
+  unfold toFact
+  grind
 
 /-- Converting a `FunctionFreeFact` to a `Fact` and back yields the initial `FunctionFreeFact`. -/
+@[simp, grind =]
 theorem toFunctionFreeFact_after_toFact_is_id (f : FunctionFreeFact sig) : f.toFact.toFunctionFreeFact (f.toFact_isFunctionFree) = f := by
   unfold toFact
   unfold Fact.toFunctionFreeFact
@@ -448,7 +455,7 @@ theorem toFunctionFreeFact_after_toFact_is_id (f : FunctionFreeFact sig) : f.toF
   constructor
   . simp
   . rw [List.map_attach_eq_pmap, List.pmap_map]
-    simp [GroundTerm.toConst, GroundTerm.const]
+    simp
 
 end FunctionFreeFact
 
@@ -457,24 +464,18 @@ namespace Fact
 variable {sig : Signature} [DecidableEq sig.P] [DecidableEq sig.C] [DecidableEq sig.V]
 
 /-- Converting a `Fact` to a `FunctionFreeFact` and back yields the initial `Fact`. -/
+@[simp, grind =]
 theorem toFact_after_toFunctionFreeFact_is_id (f : Fact sig) (isFunctionFree : f.isFunctionFree) : (f.toFunctionFreeFact isFunctionFree).toFact = f := by
   unfold toFunctionFreeFact
   unfold FunctionFreeFact.toFact
-  simp
+  simp only
   rw [GeneralizedAtom.mk.injEq]
   constructor
   . simp
-  . simp only [List.map_attach_eq_pmap]
+  . rw [List.map_attach_eq_pmap]
     apply List.ext_get
     . simp
-    intro n _ _
-    simp
-    specialize isFunctionFree f.terms[n] (by simp)
-    rcases isFunctionFree with ⟨c, isFunctionFree⟩
-    simp only [isFunctionFree]
-    unfold GroundTerm.const
-    unfold GroundTerm.toConst
-    simp
+    . grind
 
 end Fact
 
@@ -494,39 +495,48 @@ namespace FactSet
 variable {sig : Signature} [DecidableEq sig.P] [DecidableEq sig.C] [DecidableEq sig.V]
 
 /-- The predicate symbols of a `FactSet` are the predicate symbols from all facts. -/
+@[expose]
 def predicates (fs : FactSet sig) : Set sig.P := fun p => ∃ f, f ∈ fs ∧ f.predicate = p
 
 /-- The terms of a `FactSet` are the terms from all facts. -/
+@[expose]
 def terms (fs : FactSet sig) : Set (GroundTerm sig) := fun t => ∃ f, f ∈ fs ∧ t ∈ f.terms
 
 /-- The constants of a `FactSet` are the constants from all facts. -/
+@[expose]
 def constants (fs : FactSet sig) : Set sig.C := fun c => ∃ f, f ∈ fs ∧ c ∈ f.constants
 
 /-- The function symbols of a `FactSet` are the function symbols from all facts. -/
+@[expose]
 def function_symbols (fs : FactSet sig) : Set (SkolemFS sig) := fun func => ∃ f, f ∈ fs ∧ func ∈ f.function_symbols
 
 /-- A `FactSet` is function free if all of its facts are. -/
+@[expose]
 def isFunctionFree (fs : FactSet sig) : Prop := ∀ f, f ∈ fs -> f.isFunctionFree
 
 /-- When converting a list to a `FactSet`, the terms remain the same. -/
+@[simp, grind =]
 theorem mem_terms_toSet {l : List (Fact sig)} : ∀ t, t ∈ FactSet.terms (l.toSet) ↔ t ∈ l.flatMap GeneralizedAtom.terms := by
   intro t; rw [List.mem_flatMap]
-  constructor <;> (rintro ⟨f, f_mem, t_mem⟩; exists f)
+  constructor <;> (intro ⟨f, f_mem, t_mem⟩; exists f; grind)
 
 /-- The a `FactSet` is a subset of another, then their terms share this subset relation. -/
+@[grind ->]
 theorem terms_subset_of_subset {fs1 fs2 : FactSet sig} : fs1 ⊆ fs2 -> fs1.terms ⊆ fs2.terms := by
-  rintro sub t ⟨f, f_mem, t_mem⟩; exists f; exact ⟨sub _ f_mem, t_mem⟩
+  intro sub t ⟨f, f_mem, t_mem⟩; exists f; exact ⟨sub _ f_mem, t_mem⟩
 
 /-- The terms of the union of two `FactSet`s are the union of the terms of both sets. -/
+@[simp, grind =]
 theorem terms_union {fs1 fs2 : FactSet sig} : (fs1 ∪ fs2).terms = fs1.terms ∪ fs2.terms := by
-  apply Set.ext
-  intro t; constructor
+  ext t
+  constructor
   . rintro ⟨f, f_mem, t_mem⟩; cases f_mem with | inl f_mem => apply Or.inl; exists f | inr f_mem => apply Or.inr; exists f
   . intro t_mem; cases t_mem with
-    | inl t_mem => rcases t_mem with ⟨f, f_mem, t_mem⟩; exists f; simp only [t_mem, and_true]; exact Or.inl f_mem
-    | inr t_mem => rcases t_mem with ⟨f, f_mem, t_mem⟩; exists f; simp only [t_mem, and_true]; exact Or.inr f_mem
+    | inl t_mem => rcases t_mem with ⟨f, f_mem, t_mem⟩; exists f; grind
+    | inr t_mem => rcases t_mem with ⟨f, f_mem, t_mem⟩; exists f; grind
 
 /-- If a `FactSet` is finite, so are its terms. -/
+@[grind ->]
 theorem terms_finite_of_finite (fs : FactSet sig) (finite : fs.finite) : fs.terms.finite := by
   rcases finite with ⟨l, nodup, finite⟩
   exists (l.map GeneralizedAtom.terms).flatten.eraseDupsKeepRight
@@ -540,37 +550,33 @@ theorem terms_finite_of_finite (fs : FactSet sig) (finite : fs.finite) : fs.term
       rcases in_l with ⟨terms, ex_f, e_in_terms⟩
       rcases ex_f with ⟨f, f_in_l, terms_eq⟩
       exists f
-      constructor
-      . rw [← finite]; exact f_in_l
-      . rw [terms_eq]; exact e_in_terms
+      grind
     . intro in_fs
       unfold FactSet.terms at in_fs
       simp [List.mem_eraseDupsKeepRight, List.mem_flatten]
       rcases in_fs with ⟨f, f_in_fs, e_in_f⟩
       exists f.terms
-      constructor
-      . exists f
-        constructor
-        . rw [finite]; exact f_in_fs
-        . rfl
-      . exact e_in_f
+      grind
 
 /-- When converting a list to a `FactSet`, the constants remain the same. -/
+@[simp, grind =]
 theorem mem_constants_toSet {l : List (Fact sig)} : ∀ c, c ∈ FactSet.constants (l.toSet) ↔ c ∈ l.flatMap Fact.constants := by
   intro t; rw [List.mem_flatMap]
-  constructor <;> (rintro ⟨f, f_mem, t_mem⟩; exists f)
+  constructor <;> (rintro ⟨f, f_mem, t_mem⟩; exists f; grind)
 
 /-- The constants of the union of two `FactSet`s are the union of the constants of both sets. -/
+@[simp, grind =]
 theorem constants_union {fs1 fs2 : FactSet sig} : (fs1 ∪ fs2).constants = fs1.constants ∪ fs2.constants := by
   -- NOTE: same proof as terms_union
-  apply Set.ext
-  intro t; constructor
+  ext t
+  constructor
   . rintro ⟨f, f_mem, t_mem⟩; cases f_mem with | inl f_mem => apply Or.inl; exists f | inr f_mem => apply Or.inr; exists f
   . intro t_mem; cases t_mem with
-    | inl t_mem => rcases t_mem with ⟨f, f_mem, t_mem⟩; exists f; simp only [t_mem, and_true]; exact Or.inl f_mem
-    | inr t_mem => rcases t_mem with ⟨f, f_mem, t_mem⟩; exists f; simp only [t_mem, and_true]; exact Or.inr f_mem
+    | inl t_mem => rcases t_mem with ⟨f, f_mem, t_mem⟩; exists f; grind
+    | inr t_mem => rcases t_mem with ⟨f, f_mem, t_mem⟩; exists f; grind
 
 /-- If a `FactSet` is finite, so are its constants. -/
+@[grind ->]
 theorem constants_finite_of_finite (fs : FactSet sig) (fin : fs.finite) : fs.constants.finite := by
   rcases fin with ⟨l, _, l_eq⟩
   exists (l.flatMap Fact.constants).eraseDupsKeepRight
@@ -591,6 +597,7 @@ theorem constants_finite_of_finite (fs : FactSet sig) (fin : fs.finite) : fs.con
       exists f
 
 /-- A `FactSet` is finite if both its predicates and terms are. This holds since the fact set must be a subset of all facts that can possibly be constructed using the prediactes and terms available. This overapproximation is easily shown to be finite. -/
+@[grind ->]
 theorem finite_of_preds_finite_of_terms_finite (fs : FactSet sig) : fs.predicates.finite -> fs.terms.finite -> fs.finite := by
   intro preds_fin terms_fin
   rcases preds_fin with ⟨preds, _, preds_eq⟩
@@ -614,17 +621,7 @@ theorem finite_of_preds_finite_of_terms_finite (fs : FactSet sig) : fs.predicate
       rw [List.mem_eraseDupsKeepRight]
       simp only [List.mem_flatMap, List.mem_map, List.mem_attach, true_and, Subtype.exists]
       constructor
-      . intro h
-        rcases h with ⟨pred, pred_mem, ts, ts_mem, f_eq⟩
-        rw [← f_eq]
-        constructor
-        . rw [preds_eq] at pred_mem
-          exact pred_mem
-        . rw [mem_all_lists_of_length] at ts_mem
-          intro t t_mem
-          rw [← terms_eq]
-          apply ts_mem.right
-          exact t_mem
+      . intro _; constructor <;> grind
       . intro h
         rcases h with ⟨pred_mem, ts_mem⟩
         exists f.predicate
@@ -658,10 +655,7 @@ theorem list_of_facts_for_list_of_terms {ts : List (GroundTerm sig)} {fs : FactS
       cases mem with
       | inl mem => rw [mem]; exact f_mem
       | inr mem => apply l_sub; rw [List.mem_toSet]; exact mem
-    . intro s; rw [List.mem_cons, List.flatMap_cons, List.mem_append]
-      intro s_mem; cases s_mem with
-      | inl s_mem => apply Or.inl; rw [s_mem]; exact t_mem
-      | inr s_mem => apply Or.inr; apply ts_sub; exact s_mem
+    . grind
 
 end FactSet
 
@@ -730,31 +724,21 @@ def constants (db : Database sig) : { C : Set sig.C // C.finite } := ⟨
 ⟩
 
 /-- When converting a `Database` to a `FactSet`, the constants remain the same. -/
+@[simp, grind =]
 theorem toFactSet_constants_same (db : Database sig) : db.toFactSet.val.constants = db.constants.val := by
   unfold toFactSet
   unfold constants
   unfold FactSet.constants
   simp only
-  apply Set.ext
-  intro c
+  ext c
   constructor
   . intro h
     rcases h with ⟨f, f_mem, c_mem⟩
+    unfold Fact.constants at c_mem
     rcases f_mem with ⟨f', f'_mem, f_eq⟩
+    unfold FunctionFreeFact.toFact at f_eq
     exists f'
-    constructor
-    . exact f'_mem
-    . unfold Fact.constants at c_mem
-      rw [List.mem_flatMap] at c_mem
-      rcases c_mem with ⟨t, t_mem, c_mem⟩
-      rw [← f_eq] at t_mem
-      unfold FunctionFreeFact.toFact at t_mem
-      rw [List.mem_map] at t_mem
-      rcases t_mem with ⟨d, d_mem, t_eq⟩
-      rw [← t_eq] at c_mem
-      rw [GroundTerm.constants_const, List.mem_singleton] at c_mem
-      rw [c_mem]
-      exact d_mem
+    grind
   . intro h
     rcases h with ⟨f, f_mem, c_mem⟩
     exists f.toFact
@@ -762,12 +746,7 @@ theorem toFactSet_constants_same (db : Database sig) : db.toFactSet.val.constant
     . exists f
     . unfold FunctionFreeFact.toFact
       unfold Fact.constants
-      rw [List.mem_flatMap]
-      exists GroundTerm.const c
-      constructor
-      . rw [List.mem_map]
-        exists c
-      . simp [GroundTerm.constants_const]
+      grind
 
 end Database
 
@@ -789,6 +768,7 @@ namespace KnowledgeBase
 variable {sig : Signature} [DecidableEq sig.P] [DecidableEq sig.C] [DecidableEq sig.V]
 
 /-- A `KnowledgeBase` is determinstic if the underlying `RuleSet` is. -/
+@[expose]
 def isDeterministic (kb : KnowledgeBase sig) : Prop := kb.rules.isDeterministic
 
 end KnowledgeBase
