ExistentialRules/AtomsAndFacts/SubstitutionsAndHomomorphisms.lean
@@ -1,6 +1,8 @@
+module
+
 import BasicLeanDatastructures.List.Basic
 
-import ExistentialRules.AtomsAndFacts.Basic
+public import ExistentialRules.AtomsAndFacts.Basic
 
 /-!
 # Substitutions and other mappings on Terms
@@ -8,6 +10,8 @@ import ExistentialRules.AtomsAndFacts.Basic
 In this file, we define mainly `GroundSubstitution` and `GroundTermMapping`. The latter is used to define homomorphisms on `FactSet`s.
 Both kinds of mapping are based on a (very general) `TermMapping`.
 -/
+
+public section
 
 section TermMapping
 
@@ -26,6 +30,7 @@ namespace TermMapping
 variable {sig : Signature} [DecidableEq sig.P]
 
 /-- A `TermMapping` is applied to a `GeneralizedAtom` by simply applying it to each term. -/
+@[expose]
 def apply_generalized_atom (h : TermMapping S T) (a : GeneralizedAtom sig S) : GeneralizedAtom sig T := {
   predicate := a.predicate
   terms := a.terms.map h
@@ -41,17 +46,18 @@ def apply_generalized_atom_set (h : TermMapping S T) (s : Set (GeneralizedAtom s
   s.map h.apply_generalized_atom
 
 /-- Applying a `TermMapping` to a `GeneralizedAtom` does not change the number of terms.-/
+@[simp, grind =]
 theorem length_terms_apply_generalized_atom (h : TermMapping S T) (a : GeneralizedAtom sig S) :
     (h.apply_generalized_atom a).terms.length = a.terms.length := by
   simp [apply_generalized_atom]
 
 /-- We can split the application of a composed `TermMapping` on an atom. -/
-theorem apply_generalized_atom_compose (g : TermMapping S T) (h : TermMapping T U) : apply_generalized_atom (sig := sig) (h ∘ g) = (apply_generalized_atom h) ∘ (apply_generalized_atom g) := by
-  apply funext
-  intro a
-  simp [apply_generalized_atom]
+theorem apply_generalized_atom_compose (g : TermMapping S T) (h : TermMapping T U) :
+    apply_generalized_atom (sig := sig) (h ∘ g) = (apply_generalized_atom h) ∘ (apply_generalized_atom g) := by
+  ext a; simp [apply_generalized_atom]
 
 /-- We can split the application of a composed `TermMapping` on an atom. -/
+@[simp, grind =]
 theorem apply_generalized_atom_compose' (g : TermMapping S T) (h : TermMapping T U) : ∀ (a : GeneralizedAtom sig S), apply_generalized_atom (h ∘ g) a = (apply_generalized_atom h) (apply_generalized_atom g a) := by
   intro a
   rw [← Function.comp_apply (f := h.apply_generalized_atom)]
@@ -64,8 +70,7 @@ theorem apply_generalized_atom_congr_left (g h : TermMapping S T) (a : Generaliz
   rw [GeneralizedAtom.mk.injEq]
   constructor
   . rfl
-  . apply List.map_congr_left
-    exact same
+  . apply List.map_congr_left; exact same
 
 /-- Applying a `TermMapping` on a `GeneralizedAtom` is the identity if the mapping is the identity on each term. -/
 theorem apply_generalized_atom_eq_self_of_id_on_terms (h : TermMapping T T) (a : GeneralizedAtom sig T) (id_on_terms : ∀ t ∈ a.terms, h t = t) :
@@ -73,69 +78,65 @@ theorem apply_generalized_atom_eq_self_of_id_on_terms (h : TermMapping T T) (a :
   rw [GeneralizedAtom.mk.injEq]
   constructor
   . rfl
-  . apply List.map_id_of_id_on_all_mem
-    exact id_on_terms
+  . apply List.map_id_of_id_on_all_mem; exact id_on_terms
+
+/-- Unfold the defintiion of apply_generalized_atom_list for membership. -/
+@[simp, grind =]
+theorem mem_apply_generalized_atom_list {h : TermMapping S T} {l : List (GeneralizedAtom sig S)} {a : GeneralizedAtom sig T} :
+    a ∈ apply_generalized_atom_list h l ↔ ∃ b ∈ l, a = h.apply_generalized_atom b := by
+  unfold apply_generalized_atom_list
+  grind
 
 /-- We can split the application of a composed `TermMapping` on a list of atoms. -/
-theorem apply_generalized_atom_list_compose (g : TermMapping S T) (h : TermMapping T U) : apply_generalized_atom_list (sig := sig) (h ∘ g) = (apply_generalized_atom_list h) ∘ (apply_generalized_atom_list g) := by
-  apply funext
-  intro l
+theorem apply_generalized_atom_list_compose (g : TermMapping S T) (h : TermMapping T U) :
+    apply_generalized_atom_list (sig := sig) (h ∘ g) = (apply_generalized_atom_list h) ∘ (apply_generalized_atom_list g) := by
+  ext l
   unfold apply_generalized_atom_list
   rw [Function.comp_apply, List.map_map]
   rw [apply_generalized_atom_compose]
 
 /-- We can split the application of a composed `TermMapping` on a list of atoms. -/
-theorem apply_generalized_atom_list_compose' (g : TermMapping S T) (h : TermMapping T U) : ∀ l : List (GeneralizedAtom sig S), apply_generalized_atom_list (h ∘ g) l = (apply_generalized_atom_list h) (apply_generalized_atom_list g l) := by
+@[simp, grind =]
+theorem apply_generalized_atom_list_compose' (g : TermMapping S T) (h : TermMapping T U) :
+    ∀ l : List (GeneralizedAtom sig S), apply_generalized_atom_list (h ∘ g) l = (apply_generalized_atom_list h) (apply_generalized_atom_list g l) := by
   intro l
   rw [← Function.comp_apply (f := h.apply_generalized_atom_list)]
   rw [← apply_generalized_atom_list_compose]
 
-/-- We can split the application of a composed `TermMapping` on a set of atoms. -/
-theorem apply_generalized_atom_set_compose (g : TermMapping S T) (h : TermMapping T U) : apply_generalized_atom_set (sig := sig) (h ∘ g) = (apply_generalized_atom_set h) ∘ (apply_generalized_atom_set g) := by
-  apply funext
-  intro s
-  apply Set.ext
-  intro a
-  constructor
-  . intro pre
-    rcases pre with ⟨a', a'_mem, a'_eq⟩
-    rw [apply_generalized_atom_compose, Function.comp_apply] at a'_eq
-    exists g.apply_generalized_atom a'
-    constructor
-    . exists a'
-    . exact a'_eq
-  . intro pre
-    rcases pre with ⟨a', a'_mem, a'_eq⟩
-    rcases a'_mem with ⟨a'', a''_mem, a''_eq⟩
-    exists a''
-    constructor
-    . exact a''_mem
-    . rw [apply_generalized_atom_compose, Function.comp_apply]
-      rw [a''_eq, a'_eq]
+/-- Unfold the defintiion of apply_generalized_atom_set for membership. -/
+@[simp, grind =]
+theorem mem_apply_generalized_atom_set {h : TermMapping S T} {s : Set (GeneralizedAtom sig S)} {a : GeneralizedAtom sig T} :
+    a ∈ apply_generalized_atom_set h s ↔ ∃ b ∈ s, a = h.apply_generalized_atom b := by
+  unfold apply_generalized_atom_set
+  rw [Set.mem_map]
+  grind
 
 /-- We can split the application of a composed `TermMapping` on a set of atoms. -/
-theorem apply_generalized_atom_set_compose' (g : TermMapping S T) (h : TermMapping T U) : ∀ s : Set (GeneralizedAtom sig S), apply_generalized_atom_set (h ∘ g) s = (apply_generalized_atom_set h) (apply_generalized_atom_set g s) := by
-  intro l
-  rw [← Function.comp_apply (f := h.apply_generalized_atom_set)]
-  rw [← apply_generalized_atom_set_compose]
+theorem apply_generalized_atom_set_compose (g : TermMapping S T) (h : TermMapping T U) :
+  apply_generalized_atom_set (sig := sig) (h ∘ g) = (apply_generalized_atom_set h) ∘ (apply_generalized_atom_set g) := by grind
+
+/-- We can split the application of a composed `TermMapping` on a set of atoms. -/
+@[simp, grind =]
+theorem apply_generalized_atom_set_compose' (g : TermMapping S T) (h : TermMapping T U) :
+  ∀ s : Set (GeneralizedAtom sig S), apply_generalized_atom_set (h ∘ g) s = (apply_generalized_atom_set h) (apply_generalized_atom_set g s) := by grind
 
 /-- Applying a `TermMapping` to both an atom and a set of atoms retains membership of the atom in the set. -/
+@[grind =>]
 theorem apply_generalized_atom_mem_apply_generalized_atom_set
     (h : TermMapping S T) (a : GeneralizedAtom sig S) (as : Set (GeneralizedAtom sig S)) :
     a ∈ as -> h.apply_generalized_atom a ∈ h.apply_generalized_atom_set as := by
   intro a_mem
+  simp only [apply_generalized_atom_set, Set.mem_map]
   exists a
 
 /-- Applying the same `TermMapping` to two sets of atoms retains their subset relation. -/
+@[grind =>]
 theorem apply_generalized_atom_set_subset_of_subset (h : TermMapping S T) (as bs : Set (GeneralizedAtom sig S)) :
     as ⊆ bs -> h.apply_generalized_atom_set as ⊆ h.apply_generalized_atom_set bs := by
   intro subset
   intro a a_mem
-  rcases a_mem with ⟨a', a'_mem, a'_eq⟩
-  rw [← a'_eq]
-  apply apply_generalized_atom_mem_apply_generalized_atom_set
-  apply subset
-  exact a'_mem
+  simp only [apply_generalized_atom_set, Set.mem_map] at a_mem
+  grind
 
 /-- When mapping a set of atoms that results from the list, we can instead map on the list and then convert to the set. -/
 theorem apply_generalized_atom_set_toSet {g : TermMapping S T} :
@@ -163,29 +164,29 @@ namespace GroundSubstitution
 variable {sig : Signature} [DecidableEq sig.C] [DecidableEq sig.V]
 
 /-- We lift `GroundSubstitution`s to mappings from `VarOrConst` to `GroundTerm` in the obvious way. -/
+@[expose]
 def apply_var_or_const (σ : GroundSubstitution sig) : TermMapping (VarOrConst sig) (GroundTerm sig)
-  | .var v => σ v
-  | .const c => GroundTerm.const c
+| .var v => σ v
+| .const c => GroundTerm.const c
 
 /-- We lift `GroundSubstitution`s to mappings from `SkolemTerm` to `GroundTerm` in the obvious way. -/
+@[expose]
 def apply_skolem_term (σ : GroundSubstitution sig) : TermMapping (SkolemTerm sig) (GroundTerm sig)
-  | .var v => σ v
-  | .const c => GroundTerm.const c
-  | .func fs frontier arity_ok =>
-    GroundTerm.func fs (frontier.map (fun fv => σ fv)) (by
-      rw [List.length_map]
-      exact arity_ok
-    )
+| .var v => σ v
+| .const c => GroundTerm.const c
+| .func fs frontier arity_ok =>
+  GroundTerm.func fs (frontier.map (fun fv => σ fv)) (by
+    rw [List.length_map]
+    exact arity_ok
+  )
 
 /-- On functional `SkolemTerm`s that share the same frontier, applying a `GroundSubstitution` is injective. -/
+@[grind ->]
 theorem apply_skolem_term_injective_on_func_of_frontier_eq
     (subs : GroundSubstitution sig) (s t : SkolemTerm sig)
     (hs : s = SkolemTerm.func a frontier arity_a) (ht : t = SkolemTerm.func b frontier arity_b) :
     subs.apply_skolem_term s = subs.apply_skolem_term t -> s = t := by
-  simp only [hs, ht, apply_skolem_term]
-  intro h
-  simp only [GroundTerm.func, Subtype.mk.injEq, FiniteTree.inner.injEq, and_true] at h
-  simp [h]
+  rw [hs, ht]; simp [apply_skolem_term]
 
 variable [DecidableEq sig.P]
 
@@ -220,6 +221,8 @@ namespace GroundTermMapping
 
 variable {sig : Signature} [DecidableEq sig.C] [DecidableEq sig.V]
 
+/-- Every constant is mapped to itself. -/
+@[expose]
 def isIdOnConstants (h : GroundTermMapping sig) : Prop := ∀ {c}, h (.const c) = .const c
 
 variable [DecidableEq sig.P]
@@ -231,27 +234,36 @@ abbrev applyFact (h : GroundTermMapping sig) : Fact sig -> Fact sig := h.apply_g
 abbrev applyFactSet (h : GroundTermMapping sig) : FactSet sig -> FactSet sig := h.apply_generalized_atom_set
 
 /-- A `GroundTermMapping` is a homomorphisms from `FactSet` A to B if each constant is mapped to itself and mapping A results in a subset of B. -/
+@[expose]
 def isHomomorphism (h : GroundTermMapping sig) (A B : FactSet sig) : Prop :=
   isIdOnConstants h ∧ (h.applyFactSet A ⊆ B)
 
+/-- Unfold the `applyFactSet` definition for membership. -/
+@[simp, grind =]
+theorem mem_applyFactSet {h : GroundTermMapping sig} {fs : FactSet sig} {f : Fact sig} : f ∈ h.applyFactSet fs ↔ ∃ e ∈ fs, f = h.applyFact e := by grind
+
 /-- The terms in a mapped `FactSet` are the same as the mapped terms from the original `FactSet`. -/
+@[simp, grind =]
 theorem terms_applyFactSet {h : GroundTermMapping sig} {fs : FactSet sig} : (h.applyFactSet fs).terms = fs.terms.map h := by
-  apply Set.ext; intro t
+  ext t
+  unfold FactSet.terms
+  simp only [Set.mem_map, mem_applyFactSet]
   constructor
-  . rintro ⟨f, ⟨f', f'_mem, f_eq⟩, t_mem⟩
-    rw [← f_eq] at t_mem
+  . intro ⟨f, ⟨f', f'_mem, f_eq⟩, t_mem⟩
+    rw [f_eq] at t_mem
     simp only [TermMapping.apply_generalized_atom, List.mem_map] at t_mem
     rcases t_mem with ⟨t', t'_mem, t_eq⟩
     rw [← t_eq]
     exists t'; simp only [and_true]
     exists f'
-  . rintro ⟨t', ⟨f', f'_mem, t'_mem⟩, t_eq⟩
+  . intro ⟨t', ⟨f', f'_mem, t'_mem⟩, t_eq⟩
     rw [← t_eq]
     exists h.applyFact f'; constructor
-    . apply TermMapping.apply_generalized_atom_mem_apply_generalized_atom_set; exact f'_mem
+    . exists f'
     . simp only [applyFact, TermMapping.apply_generalized_atom]; apply List.mem_map_of_mem; exact t'_mem
 
 /-- We can compose homomorphisms. That is, given a homomorphism from A to B and from B to C, we can combine both to obtain a homomorphisms from A to C. -/
+@[grind ->]
 theorem isHomomorphism_compose (g h : GroundTermMapping sig) (A B C : FactSet sig) :
     g.isHomomorphism A B -> h.isHomomorphism B C -> isHomomorphism (h ∘ g) A C := by
   intro g_hom h_hom
@@ -259,10 +271,12 @@ theorem isHomomorphism_compose (g h : GroundTermMapping sig) (A B C : FactSet si
   . intro c
     rw [Function.comp_apply, g_hom.left, h_hom.left]
   . unfold applyFactSet
-    rw [TermMapping.apply_generalized_atom_set_compose]
+    rw [TermMapping.apply_generalized_atom_set_compose']
     intro f f_mem_compose
+    rw [TermMapping.mem_apply_generalized_atom_set] at f_mem_compose
     rcases f_mem_compose with ⟨f', f'_mem, f'_eq⟩
     apply h_hom.right
+    rw [mem_applyFactSet]
     exists f'
     constructor
     . apply g_hom.right
@@ -286,17 +300,14 @@ variable {sig : Signature} [DecidableEq sig.C] [DecidableEq sig.V]
 
 /-- The application of a composed substitution on a `VarOrConst` can be split if the involved `GroundTermMapping` maps the `VarOrConst` to itself, in the case where it is a constant. -/
 theorem GroundSubstitution.apply_var_or_const_compose (s : GroundSubstitution sig) (h : GroundTermMapping sig) :
-    ∀ (voc : VarOrConst sig), (∀ d, voc = VarOrConst.const d -> h (GroundTerm.const d) = GroundTerm.const d) -> GroundSubstitution.apply_var_or_const (h ∘ s) voc = h (s.apply_var_or_const voc) := by
+    ∀ (voc : VarOrConst sig), (∀ d, voc = VarOrConst.const d -> h (GroundTerm.const d) = GroundTerm.const d) ->
+    GroundSubstitution.apply_var_or_const (h ∘ s) voc = h (s.apply_var_or_const voc) := by
   intro voc id_on_const
   unfold GroundSubstitution.apply_var_or_const
-  cases voc with
-  | var v => simp
-  | const c =>
-    simp only
-    rw [id_on_const]
-    rfl
+  cases voc <;> simp [id_on_const]
 
 /-- This is a special case of the above theorem where the `GroundTermMapping` is simply the id on all constants. -/
+@[simp, grind =]
 theorem GroundSubstitution.apply_var_or_const_compose_of_isIdOnConstants (s : GroundSubstitution sig)
     (h : GroundTermMapping sig) (id_on_const : h.isIdOnConstants) :
     GroundSubstitution.apply_var_or_const (h ∘ s) = h ∘ s.apply_var_or_const := by
@@ -310,32 +321,30 @@ variable [DecidableEq sig.P]
 
 /-- The application of a composed substitution on a `FunctionFreeAtom` can be split if the involved `GroundTermMapping` maps all constants from the atom to themselves. -/
 theorem GroundSubstitution.apply_function_free_atom_compose (s : GroundSubstitution sig) (h : GroundTermMapping sig) :
-    ∀ (a : FunctionFreeAtom sig), (∀ d ∈ a.constants, h (GroundTerm.const d) = GroundTerm.const d) -> GroundSubstitution.apply_function_free_atom (h ∘ s) a = h.applyFact (s.apply_function_free_atom a) := by
+    ∀ (a : FunctionFreeAtom sig), (∀ d ∈ a.constants, h (GroundTerm.const d) = GroundTerm.const d) ->
+    GroundSubstitution.apply_function_free_atom (h ∘ s) a = h.applyFact (s.apply_function_free_atom a) := by
   intro a id_on_const
   unfold GroundTermMapping.applyFact
   rw [← TermMapping.apply_generalized_atom_compose']
   apply TermMapping.apply_generalized_atom_congr_left
   intro voc voc_mem
   apply apply_var_or_const_compose
-  intro d d_eq
-  apply id_on_const
-  unfold FunctionFreeAtom.constants
-  apply VarOrConst.mem_filterConsts_of_const
-  rw [d_eq] at voc_mem
-  exact voc_mem
+  grind
 
 /-- This is a special case of the above theorem where the `GroundTermMapping` is simply the id on all constants. -/
-theorem GroundSubstitution.apply_function_free_atom_compose_of_isIdOnConstants (s : GroundSubstitution sig) (h : GroundTermMapping sig) (id_on_const : h.isIdOnConstants) :
+@[simp, grind =]
+theorem GroundSubstitution.apply_function_free_atom_compose_of_isIdOnConstants
+    (s : GroundSubstitution sig) (h : GroundTermMapping sig) (id_on_const : h.isIdOnConstants) :
     GroundSubstitution.apply_function_free_atom (h ∘ s) = h.applyFact ∘ s.apply_function_free_atom := by
-  apply funext
-  intro a
+  ext a
   apply apply_function_free_atom_compose
   intros
   exact id_on_const
 
 /-- The application of a composed substitution on a `FunctionFreeConjunction` can be split if the involved `GroundTermMapping` maps all constants from the conjucntion to themselves. -/
 theorem GroundSubstitution.apply_function_free_conj_compose (s : GroundSubstitution sig) (h : GroundTermMapping sig) :
-    ∀ (ffc : FunctionFreeConjunction sig), (∀ d ∈ ffc.consts, h (GroundTerm.const d) = GroundTerm.const d) -> GroundSubstitution.apply_function_free_conj (h ∘ s) ffc = h.apply_generalized_atom_list (s.apply_function_free_conj ffc) := by
+    ∀ (ffc : FunctionFreeConjunction sig), (∀ d ∈ ffc.consts, h (GroundTerm.const d) = GroundTerm.const d) ->
+    GroundSubstitution.apply_function_free_conj (h ∘ s) ffc = h.apply_generalized_atom_list (s.apply_function_free_conj ffc) := by
   intro ffc id_on_const
   unfold GroundSubstitution.apply_function_free_conj TermMapping.apply_generalized_atom_list
   rw [List.map_map]
@@ -343,10 +352,12 @@ theorem GroundSubstitution.apply_function_free_conj_compose (s : GroundSubstitut
   intro f f_mem
   rw [← apply_function_free_atom.eq_def, apply_function_free_atom_compose]
   . rfl
-  . intro d d_mem; apply id_on_const; simp only [FunctionFreeConjunction.consts, List.mem_flatMap]; exists f
+  . grind
 
 /-- This is a special case of the above theorem where the `GroundTermMapping` is simply the id on all constants. -/
-theorem GroundSubstitution.apply_function_free_conj_compose_of_isIdOnConstants (s : GroundSubstitution sig) (h : GroundTermMapping sig) (id_on_const : h.isIdOnConstants) :
+@[simp, grind =]
+theorem GroundSubstitution.apply_function_free_conj_compose_of_isIdOnConstants
+    (s : GroundSubstitution sig) (h : GroundTermMapping sig) (id_on_const : h.isIdOnConstants) :
     GroundSubstitution.apply_function_free_conj (h ∘ s) = h.apply_generalized_atom_list ∘ s.apply_function_free_conj := by
   apply funext
   intro ffc
